src/cbor/pulse/CBOR.Pulse.API.Det.Dummy.fsti
@@ -1,0 +1,6 @@
+module CBOR.Pulse.API.Det.Dummy
+
+module T = CBOR.Pulse.API.Det.Type
+
+inline_for_extraction
+val dummy_cbor_det_t (_: unit) : T.cbor_det_t
