src/cbor/pulse/raw/everparse/CBOR.Pulse.API.Det.C.fst
@@ -179,7 +179,7 @@ let cbor_det_map_entry_match = Impl.cbor_det_map_entry_match
 let cbor_det_mk_map_entry = Impl.cbor_det_mk_map_entry
 
 let cbor_det_mk_map_from_array : mk_map_from_array_t cbor_det_match cbor_det_map_entry_match =
-  mk_map_from_array (mk_map_from_ref (CBOR.Pulse.API.Det.Type.dummy_cbor_det_t ()) (Impl.cbor_det_mk_map_gen ()))
+  mk_map_from_array (mk_map_from_ref (CBOR.Pulse.API.Det.Dummy.dummy_cbor_det_t ()) (Impl.cbor_det_mk_map_gen ()))
 
 ghost fn map_gen_post_to_array
   (#t1 #t2: Type0)
